src/theory/tools/wp/bin_hoare_logic_test_AVScript.sml
@@ -1,0 +1,457 @@
+open HolKernel Parse boolLib bossLib;
+
+open bir_programTheory;
+open bir_auxiliaryTheory;
+open bin_hoare_logicTheory;
+open bir_program_multistep_propsTheory;
+open bir_program_blocksTheory;
+
+open bin_hoare_logicLib;
+
+open HolBACoreSimps;
+
+val _ = new_theory "bin_hoare_logic_test_AV";
+
+(*
+(* Executing till a certain set of labels is useful as well. Since we might loop
+   outside this set of labels, infinite runs are possible. *)
+val bir_exec_to_labels_n_def = Define `
+  bir_exec_to_labels_n ls p state n =
+  bir_exec_steps_GEN (F, \pc. (pc.bpc_index = 0) /\ (pc.bpc_label IN ls)) p state (SOME n)`
+
+val bir_exec_to_labels_def = Define `
+  bir_exec_to_labels ls p state = bir_exec_to_labels_n ls p state 1`
+*)
+
+(*
+Datatype `bin_model_t =
+  <|(* A function to obtain a state option from a state via
+     * execution (transition) *)
+    trs : 'a -> 'a option;
+    (* A function to determine whether a transition between two
+     * states is OK, through using a set of labels for which
+     * execution must halt if reached, meaning they cannot be
+     * touched in any intermediate step *)
+    weak : 'a -> ('b -> bool) -> 'a -> bool;
+    (* A function to obtain the program counter from a state *)
+    pc : 'a -> 'b
+   |>`;
+
+*)
+
+(*
+val weak_model_def = Define `
+  weak_model m =
+    !ms ls ms'.
+      (m.weak ms ls ms') =
+        ?n.
+          ((n > 0) /\
+           (FUNPOW_OPT m.trs n ms = SOME ms') /\
+           ((m.pc ms') IN ls)
+          ) /\
+          !n'.
+            (((n' < n) /\ (n' > 0)) ==>
+            ?ms''.
+              (FUNPOW_OPT m.trs n' ms = SOME ms'') /\
+              (~((m.pc ms'') IN ls))
+            )`;
+*)
+
+(* TODO: bir_exec_block_n should probably return a BER_Ended or a
+ * BER_Looping... *)
+(* Try bir_exec_to_addr_label - but could cause more problems *)
+(*
+val bir_trs_def = Define `
+  bir_trs prog ms =
+  SOME (
+    SND (
+      SND (
+        SND (bir_exec_block_n prog ms 1)
+      )
+    )
+  )`;
+*)
+val bir_trs_def = Define `
+  bir_trs (prog:'a bir_program_t) ms =
+  let
+    (_, _, _, st) = bir_exec_block_n prog ms 1
+  in
+   if st.bst_status = BST_Running
+   then SOME st
+   else NONE
+`;
+
+(* TODO: Move elsewhere... *)
+val bir_get_current_statement_EMPTY =
+  store_thm("bir_get_current_statement_EMPTY",
+  ``!pc.
+      bir_get_current_statement (BirProgram []) pc = NONE``,
+
+FULL_SIMP_TAC (std_ss++holBACore_ss)
+              [bir_get_current_statement_def,
+               bir_get_program_block_info_by_label_def,
+               listTheory.INDEX_FIND_def]
+);
+
+val bir_exec_block_n_EXISTS = store_thm("bir_exec_block_n_EXISTS",
+  ``!prog ms.
+      ?a b c d.
+        bir_exec_block_n prog ms 1 = (a, b, c, d)``,
+
+REPEAT STRIP_TAC >>
+Cases_on `bir_state_is_terminated ms` >- (
+  FULL_SIMP_TAC std_ss [bir_exec_block_n_REWR_TERMINATED]
+) >>
+FULL_SIMP_TAC std_ss [bir_exec_block_n_TO_steps_GEN,
+                      bir_exec_steps_GEN_1_EQ_Ended] >>
+cheat
+(* Proof sketch from here:
+   Either the PC of state ms points to a block in prog, or it does
+   not. If it does not, we are OK, since any execution will result
+   in Failed, terminating and yielding an Ended result.
+
+   If the PC of state ms points to some block in prog, then do
+   induction the list of basic statements: For the empty list, the
+   PC must point to the ending statement. Consider the cases: if the
+   ending statement is Halt, we are OK. If the ending statement is
+   a CJmp whose condition fails to evaluate, we are OK. If the
+   ending statement jumps outside the program, we are OK, since
+   this will cause JumpOutside, which is a terminating state. In
+   the case of jumps inside the program, there exist two
+   possibilities: either jumps to other blocks (OK) or jumps to the
+   same block, which will not give a Looping result, but will make
+   pc_cond trigger.
+
+   For every basic statement in a non-empty list, we will either
+   terminate (by violating Assertions or Assumptions), in which case
+   we are OK, or we will proceed to executing the next basic
+   statement, or the ending statement (in which case the proof is
+   same as above).
+
+*)
+(* OLD:
+Cases_on `prog` >>
+Cases_on `l` >- (
+  (* Case: Empty program *)
+  (* TODO: Lemma about empty program? *)
+  FULL_SIMP_TAC std_ss [bir_exec_infinite_steps_fun_def] >>
+  EXISTS_TAC ``1:num`` >>
+  EXISTS_TAC ``0:num`` >>
+  FULL_SIMP_TAC std_ss [arithmeticTheory.FUNPOW_1,
+                        bir_exec_step_state_def,
+                        bir_exec_step_def,
+                        arithmeticTheory.FUNPOW] >>
+  CONJ_TAC >- (
+    FULL_SIMP_TAC (std_ss++holBACore_ss)
+                  [bir_state_COUNT_PC_def,
+                   bir_get_current_statement_EMPTY,
+                   bir_state_set_failed_def],
+  ) >>
+  CONJ_TAC >- (
+    FULL_SIMP_TAC (std_ss++holBACore_ss)
+                  [bir_get_current_statement_EMPTY,
+                   bir_state_set_failed_def]
+  ) >>
+  CONJ_TAC >- (
+    REPEAT STRIP_TAC >>
+    (* TODO: Lemma stating that n < 1 ==> n = 0 ??? *)
+    Cases_on `n` >| [
+      FULL_SIMP_TAC (std_ss++holBACore_ss)
+		    [arithmeticTheory.FUNPOW],
+
+      FULL_SIMP_TAC arith_ss []
+    ]
+  ) >>
+  FULL_SIMP_TAC arith_ss []
+) >>
+  (* Case: Program nonempty. *)
+  FULL_SIMP_TAC std_ss [bir_exec_infinite_steps_fun_def] >>
+  Cases_on `h` >>
+  Cases_on `l` >| [
+    (* Case: Statement list empty *)
+    EXISTS_TAC ``1:num`` >> (* First witness is 1 in both cases *)
+    FULL_SIMP_TAC std_ss [arithmeticTheory.FUNPOW_1,
+                          bir_exec_step_state_def,
+                          bir_exec_step_def] >>
+    Cases_on `bir_get_current_statement (BirProgram (bir_block_t b [] b0::t)) ms.bst_pc` >| [
+      FULL_SIMP_TAC (std_ss++holBACore_ss)
+                    [bir_state_set_failed_def,
+                     bir_state_COUNT_PC_def] >>
+      FULL_SIMP_TAC arith_ss [] >>
+      REPEAT STRIP_TAC >>
+      Cases_on `n` >| [
+	FULL_SIMP_TAC (std_ss++holBACore_ss)
+		      [arithmeticTheory.FUNPOW],
+
+	FULL_SIMP_TAC arith_ss []
+      ],
+
+      (* Case: Current statement is something *)
+      FULL_SIMP_TAC (std_ss++holBACore_ss) [bir_exec_stmt_def]
+      Induct_on `x`
+    ]
+
+    (* Case: Statement list non-empty. Needed to show that it is
+     * OK with termination on every statement, but quantifiers must
+     * be instantiated with this in mind... *)
+
+      (* Case of non-termination would also require a case split on
+       * the ending statement causing termination? *)
+  ]
+  (* Should be length of block h... *)
+  EXISTS_TAC ``((LENGTH (l:'a bir_stmt_basic_t list)) + 1):num`` >> 
+  EXISTS_TAC ``1:num`` >>
+  cheat
+*)
+);
+
+val _ = Datatype `bir_weak_state =
+    BWS_Regular bir_label_t
+  | BWS_Top
+  | BWS_Bottom
+`;
+
+val bir_get_weak_state_def = Define `
+  bir_get_weak_state bir_state =
+    if bir_state.bst_status = BST_Running
+    then BWS_Regular (bir_state.bst_pc.bpc_label)
+    else if bir_state.bst_status = BST_AssumptionViolated
+    then BWS_Top
+    else BWS_Bottom
+`;
+
+val bir_get_label_from_weak_state_def = Define `
+  bir_get_label_from_weak_state ws =
+    case ws of
+      BWS_Regular l => SOME l
+    | BWS_Top => NONE
+    | BWS_Bottom => NONE
+`;
+
+val bir_get_label_set_from_weak_state_set_no_top_def = Define `
+  bir_get_label_set_from_weak_state_set_no_top wss =
+    (IMAGE THE
+      ((IMAGE bir_get_label_from_weak_state wss) DELETE NONE)
+    )
+`;
+
+val bir_weak_trs_def = Define `
+  bir_weak_trs wss prog ms =
+    let 
+      ls = bir_get_label_set_from_weak_state_set_no_top wss
+    in
+    case (bir_exec_to_labels ls prog ms) of
+      BER_Ended _ _ _ bir_state =>
+        if ((bir_get_weak_state bir_state) IN wss)
+        then SOME bir_state
+        else NONE
+    | BER_Looping _ => NONE
+`;
+
+(* 1. Instantiate a new weak model *)
+val bir_etl_wm_def =
+  Define `bir_etl_wm (prog :'a bir_program_t) = <|
+    trs  := bir_trs prog;
+    weak := (\ms wss ms'.
+	       (bir_weak_trs wss prog ms = SOME ms')
+	    );
+    pc   := (\ms. bir_get_weak_state ms)
+  |>`;
+
+val wm_type = mk_thy_type {Tyop="bin_model_t",
+                           Thy="bin_hoare_logic",
+                           Args=[``:bir_state_t``,
+                                 ``:bir_label_t``]
+                          };
+
+val bir_wm_SS = rewrites (flatten (map type_rws [wm_type]));
+
+(* TODO: Move elsewhere... *)
+val bir_get_current_statement_NONE_stmt =
+  store_thm("bir_get_current_statement_NONE_stmt",
+  ``!prog pc.
+      (bir_get_current_statement prog pc = NONE) ==>
+      (bir_get_current_block prog pc = NONE)
+    ``,
+
+FULL_SIMP_TAC (std_ss++holBACore_ss)
+              [bir_get_current_block_def,
+               bir_get_current_statement_def] >>
+REPEAT STRIP_TAC >>
+Cases_on `bir_get_program_block_info_by_label
+            prog pc.bpc_label` >> (
+  FULL_SIMP_TAC (std_ss++holBACore_ss) []
+) >>
+Cases_on `x` >>
+Cases_on `0 = LENGTH r.bb_statements` >>
+Cases_on `0 < LENGTH r.bb_statements` >> (
+FULL_SIMP_TAC arith_ss []
+)
+);
+
+(* 2. Prove that weak_model bir_etl_wm *)
+val bir_model_is_weak = store_thm("bir_model_is_weak",
+  ``!(prog: 'a bir_program_t).
+      weak_model (bir_etl_wm prog)``,
+
+REPEAT STRIP_TAC >>
+FULL_SIMP_TAC (std_ss++bir_wm_SS)
+              [weak_model_def, bir_etl_wm_def] >>
+FULL_SIMP_TAC std_ss [bir_weak_trs_def, LET_DEF] >>
+REPEAT STRIP_TAC >>
+CASE_TAC >| [
+  (* Case 1: Result of bir_exec_to_labels is Ended *)
+  CASE_TAC >| [
+    (* Case 1A: Weak state counterpart of b is in ls *)
+    FULL_SIMP_TAC std_ss [bir_exec_to_labels_def] >>
+    IMP_RES_TAC bir_exec_to_labels_n_TO_bir_exec_block_n >>
+    EQ_TAC >| [
+      (* Part one: Assuming b = ms', show bir_trs plays nice *)
+      REPEAT DISCH_TAC >>
+      (* subsume b... *)
+      Q.PAT_X_ASSUM `b = ms'`
+                    (fn thm => FULL_SIMP_TAC std_ss [thm]) >>
+      FULL_SIMP_TAC std_ss [bir_exec_to_labels_n_def,
+                            bir_exec_steps_GEN_SOME_EQ_Ended] >>
+      EXISTS_TAC ``m:num`` >>
+      (* TODO: Make lemma... *)
+      subgoal `!prog ms m l n c_l' ms'.
+        (bir_exec_block_n prog ms m = (l,n,c_l',ms')) ==>
+        ?m'.
+        (FUNPOW_OPT (bir_trs prog) m' ms = SOME ms')` >- (
+        cheat
+      ) >>
+      FULL_SIMP_TAC (arith_ss++holBACore_ss) [] >>
+      REPEAT STRIP_TAC >>
+      (* TODO: Use bir_exec_steps_GEN_SOME_EQ_Ended and possibly
+       * bir_exec_block_n_TO_steps_GEN *)
+      cheat,
+
+      (* Part two: Assuming bir_trs plays nice, show that b = ms' *)
+      FULL_SIMP_TAC std_ss [bir_exec_to_labels_n_def] >>
+      cheat
+    ],
+
+    (* Case 1B: Weak state counterpart of b is NOT in ls *)
+    FULL_SIMP_TAC std_ss [GSYM boolTheory.IMP_DISJ_THM] >>
+    cheat
+  ],
+
+  (* Case 2: Result of bir_exec_to_labels is Looping *)
+  (* Show that weak state of ms' cannot be in ls *)
+  FULL_SIMP_TAC std_ss [GSYM boolTheory.IMP_DISJ_THM] >>
+  cheat
+]
+);
+
+
+
+
+
+
+
+
+(*
+
+
+      Cases_on `n > 0` >| [
+        (* Number of execution steps is non-zero (regular case) *)
+        (* Also use the fact that final state is Running *)
+        subgoal
+          `FUNPOW_OPT (bir_trs prog) n ms =
+             SOME (bir_exec_infinite_steps_fun prog ms n)` >- (
+          cheat
+        ) >>
+        FULL_SIMP_TAC std_ss [bir_state_COUNT_PC_def] >>
+        Cases_on `ms'.bst_status` >> (
+          FULL_SIMP_TAC (std_ss++holBACore_ss) []
+        ) >| [
+          (* Case: Final state is Running *)
+          REPEAT STRIP_TAC >>
+          FULL_SIMP_TAC std_ss [] >>
+          QSPECL_X_ASSUM ``!n'. _`` [`n'`] >>
+          REV_FULL_SIMP_TAC std_ss [] >>
+          (* TODO: Some kind of kinduction proof on n'? *)
+          (* bir_exec_infinite_steps_fun_COUNT_PCs_EQ_0 *)
+          cheat,
+
+          (* Case: JumpOutside requires this additional
+           *       simplification *)
+          REV_FULL_SIMP_TAC (std_ss++holBACore_ss) []
+        ],
+
+	(* Number of execution steps is zero *)
+	subgoal `n = 0` >- (
+	  FULL_SIMP_TAC arith_ss []
+	) >>
+	FULL_SIMP_TAC (std_ss++holBACore_ss)
+		      [bir_exec_infinite_steps_fun_REWRS2,
+		       bir_state_COUNT_PC_def] >>
+	Cases_on `ms'.bst_status` >> (
+	  FULL_SIMP_TAC (std_ss++holBACore_ss) []
+	) >| [
+	  (* Case: Final state is Running *)
+	  FULL_SIMP_TAC std_ss
+	    [bir_exec_infinite_steps_fun_COUNT_PCs_def],
+
+	  (* Case: JumpOutside requires this additional
+	   *       simplification *)
+	  REV_FULL_SIMP_TAC (std_ss++holBACore_ss) []
+	]
+      ],
+
+      REPEAT STRIP_TAC >>
+      QSPECL_X_ASSUM ``!n''. _`` [`n`] >>
+      (* TODO: What to do here??? *)
+      cheat
+    ],
+
+    (* Step 1B: Weak state of b is not in ls *)
+    FULL_SIMP_TAC std_ss [GSYM boolTheory.IMP_DISJ_THM] >>
+    REPEAT STRIP_TAC >>
+    (* You can choose between two disjuncts to prove. *)
+    (* Disjunct 1: Need to prove that for all non-zero step numbers
+     * n', repeated application of bir_trs resulting in SOME state
+     * ms' (meaning, before termination) entails that ms' is not
+     * in ls'.
+     *
+     * OK, since assumptions give that Ended was reached through
+     * termination, meaning that ls' was not encountered before
+     * terminating.
+     * *)
+    (* Disjunct 2: Need to prove that there exists a non-zero step
+     * number n'' such that if repeated application of bir_trs n''
+     * times gives SOME state ms'', then ms'' is in ls'.
+     *
+     * OK, since we can give a n'' larger than the steps leading to
+     * termination, making the antecedent always false.
+     * *)
+    cheat
+  ],
+
+  (* Case 2: Result of bir_exec_to_labels is Looping *)
+  FULL_SIMP_TAC std_ss [bir_exec_to_labels_def,
+			bir_exec_to_labels_n_def,
+			bir_exec_steps_GEN_EQ_Looping] >>
+  REPEAT STRIP_TAC >>
+  FULL_SIMP_TAC std_ss [GSYM boolTheory.IMP_DISJ_THM] >>
+  (* Choice of two disjuncts... *)
+(*
+  DISJ1_TAC >>
+  REPEAT STRIP_TAC >>
+  FULL_SIMP_TAC std_ss
+    [bir_exec_infinite_steps_COUNT_STEPS_EQ_NONE] >>
+*)
+  cheat
+]
+);
+*)
+(* These could be useful: *)
+(* bir_exec_steps_GEN_SOME_EQ_Ended *)
+(* bir_exec_steps_GEN_EQ_Ended *)
+(* bir_exec_steps_GEN_change_cond_Ended_SOME *)
+(* bir_exec_steps_GEN_1_EQ_Ended *)
+(* bir_exec_to_labels_n_TO_bir_exec_block_n *)
+(* bir_exec_block_n_TO_steps_GEN *)
+
+val _ = export_theory();
